AST for Dafny programs.

ocamllibs/src/codegen/Dafny.ml
@@ -1,0 +1,107 @@
+open Format
+open SketchTypes
+open SPretty
+
+(* Defintiion of a subset of the Dafny language for a cleaner management of
+   the proof generation. *)
+type type_simple
+type type_composed
+
+type _ dafny_basic_type =
+  | Int : type_simple dafny_basic_type
+  | Real: type_simple dafny_basic_type
+  | Bool: type_simple dafny_basic_type
+  | Bottom : type_simple dafny_basic_type
+  | Sequence: type_simple dafny_basic_type -> type_composed dafny_basic_type
+
+
+type 'a dfVar = string * 'a dafny_basic_type
+
+and 'a dfFuncDef = type_simple dfVar * 'a dfVar list
+
+and 'a dfProgram =
+  | DfFundec : 'a dfVar * _ dfVar list * _ dfExpr -> 'a dfProgram
+  | DfJoin : type_simple dfVar * _ dfVar list * _ dfExpr ->
+    type_simple dfProgram
+  | DfHom : type_simple dfVar * _ dfVar list * _ dfExpr -> type_simple dfProgram
+
+and dfHeader =
+  | DfRequire : type_simple dfExpr -> dfHeader
+  | DfEnsure : type_simple dfExpr -> dfHeader
+
+and 'a dfExpr =
+  | DfEmpty : type_composed dfExpr
+  | DfInt : int -> type_simple dfExpr
+  | DfBool : bool -> type_simple dfExpr
+
+  | DfFuncall : type_simple dfVar * 'a dfExpr list -> type_simple dfExpr
+  | DfVar : 'a dfVar -> 'a dfExpr
+  | DfSeqC : type_composed dfVar * type_simple dfExpr -> type_simple dfExpr
+  | DfSubSeq : type_composed dfVar * type_simple dfExpr -> type_composed dfExpr
+  | DfSeq : type_simple dfExpr -> type_composed dfExpr
+  | DfLen : type_composed dfExpr -> type_simple dfExpr
+
+  | DfIte : type_simple dfExpr * 'a dfExpr * 'a dfExpr -> 'a dfExpr
+
+  | DfBinop : 'a dfOp * _ dfExpr * _ dfExpr -> 'a dfExpr
+  | DfUnop : 'a dfOp * _ dfExpr -> 'a dfExpr
+
+  | DfSkExpr : skExpr -> type_simple dfExpr
+
+  | DfCalc : 'a dfExpr * 'a dfExpr * 'a dfExpr -> 'a dfExpr
+  | DfAssert : 'a dfExpr -> 'a dfExpr
+
+and 'a dfOp =
+  | DfEq : type_simple dfOp
+  | DfGeq : type_simple dfOp
+  | DfGe : type_simple dfOp
+  | DfPlus : type_simple dfOp
+  | DfMinus : type_simple dfOp
+
+  | DfConcat : type_composed dfOp
+  | DfEqS : type_simple dfOp
+
+  | DfSkBinop : symb_binop -> type_simple dfOp
+  | DfSkUnop : symb_unop -> type_simple dfOp
+
+
+let str_of_op : type a. a dfOp -> string =
+  function
+  | DfEqS -> "==" | DfEq -> "==" | DfGeq -> ">=" | DfGe -> ">"
+  | DfPlus -> "+" | DfMinus -> "-"
+  | DfConcat -> "+"
+  | DfSkUnop op -> string_of_symb_unop op
+  | DfSkBinop op -> string_of_symb_binop op
+
+let rec pp_dfexpr : type a. formatter -> a dfExpr -> unit =
+  (fun fmt ->
+     function
+     | DfEmpty -> fprintf fmt "[]"
+     | DfInt i -> fprintf fmt "%i" i
+     | DfBool b -> fprintf fmt "%b" b
+     | DfFuncall ((fname, ftype), args) ->
+       fprintf fmt "@[%s(%a)@]" fname
+         (pp_print_list ~pp_sep:(fun fmt () -> fprintf fmt ", ") pp_dfexpr) args
+     | DfVar (vname, vtype) -> fprintf fmt "%s" vname
+     | DfSeqC ((seqname, seqtype) , cell_e) ->
+       fprintf fmt "%s[%a]" seqname pp_dfexpr cell_e
+     | DfSubSeq ((seqname, seqtype), cell_e) ->
+       fprintf fmt "%s[..%a]" seqname pp_dfexpr cell_e
+     | DfSeq e -> fprintf fmt "[%a]" pp_dfexpr e
+     | DfLen e -> fprintf fmt "|%a|" pp_dfexpr e
+     | DfIte (c, e1, e2) ->
+       fprintf fmt "if@;%a@;{%a}@;else@;{%a}"
+         pp_dfexpr c  pp_dfexpr e1 pp_dfexpr e2
+     | DfBinop (op, e1, e2) ->
+       fprintf fmt "%a@;%s@;%a" pp_dfexpr e1 (str_of_op op) pp_dfexpr e2
+     | DfUnop (op, e) ->
+       fprintf fmt "%s@;%a" (str_of_op op) pp_dfexpr e
+     | DfCalc (lh, asserts, rh) ->
+       fprintf fmt "@[%a@\n=={%a}@\n%a@]"
+         pp_dfexpr lh pp_dfexpr asserts pp_dfexpr rh
+     | DfAssert e ->
+       fprintf fmt "assert(%a)" pp_dfexpr e
+     | DfSkExpr e -> pp_skexpr fmt e)
+
+let seq_minus_last s =
+  DfSubSeq (s, DfBinop (DfMinus, DfLen (DfVar s), DfInt 1))
