ocamllibs/dafny_examples/Example_0star1star.dfy
@@ -3,20 +3,22 @@ function DfLength(s: seq<int>): int
 
 function Aux_1(ar : seq<bool>): bool
 requires |ar| >= 1
-{ if |ar| == 1 then  ar[0] else  ar[0] 
+{
+  if |ar| == 1 then ar[0] else ar[0]
 }
 
 function An(ar : seq<bool>): bool
-{ if ar == [] then  true else  (ar[|ar|-1] && An(ar[..|ar|-1])) 
+{
+  if ar == [] then true else (ar[|ar|-1] && An(ar[..|ar|-1]))
 }
 
 function Bn(ar : seq<bool>): bool
-{ if ar == [] then
+{
+  if ar == [] then
     true
-   else 
-   (if (! ar[|ar|-1]) then Bn(ar[..|ar|-1]) else
-     ((ar[|ar|-1] && An(ar[..|ar|-1])) && Bn(ar[..|ar|-1])))
-   
+    else
+    (if (! ar[|ar|-1]) then Bn(ar[..|ar|-1]) else
+      (An(ar[..|ar|-1]) && Bn(ar[..|ar|-1])))
 }
 
 function Aux_1Join(leftAux_1 : bool, rightAux_1 : bool): bool
@@ -31,18 +33,24 @@ function AnJoin(leftBn : bool, leftAn : bool, rightBn : bool, rightAn : bool): b
 
 function BnJoin(leftAux_1 : bool, leftBn : bool, leftAn : bool, rightAux_1 : bool, rightBn : bool, rightAn : bool): bool
 {
-  (if rightAux_1 then (leftAn && rightBn) else
-    ((rightBn || rightAux_1) && ((! rightAn) && leftBn)))
+  (leftAn && rightBn) || ((rightBn && (! rightAux_1) && ((! rightAn) && leftBn)))
 }
 
 
+lemma BaseCaseAux_1(ar : seq<bool>, R_ar : seq<bool>)
+  requires |ar| >= 1 && |R_ar| >= 1
+  ensures Aux_1(ar + [R_ar[0]]) == Aux_1Join(Aux_1(ar), Aux_1([R_ar[0]]))
+  {}
+
 lemma HomAux_1(ar : seq<bool>, R_ar : seq<bool>)
+  requires |ar| >= 1 && |R_ar| >= 1
   ensures Aux_1(ar + R_ar) == Aux_1Join(Aux_1(ar), Aux_1(R_ar))
   {
-    if |R_ar| == 1 
+    if |R_ar| == 1
     {
     assert(ar + R_ar == ar + [R_ar[0]]);
-    
+    BaseCaseAux_1(ar, R_ar);
+
      } else {
     calc{
     Aux_1(ar + R_ar);
@@ -52,18 +60,13 @@ lemma HomAux_1(ar : seq<bool>, R_ar : seq<bool>)
   } // End else.
 } // End lemma.
 
-lemma BaseCaseAn(ar : seq<bool>)
-  ensures An(ar) == AnJoin(Bn(ar), An(ar), Bn([]), An([]))
-  {}
-
 lemma HomAn(ar : seq<bool>, R_ar : seq<bool>)
+	requires |ar| >= 1 && |R_ar| >= 1
   ensures An(ar + R_ar) == AnJoin(Bn(ar), An(ar), Bn(R_ar), An(R_ar))
   {
-    if R_ar == [] 
+    if |R_ar| == 1
     {
-    assert(ar + [] == ar);
-    BaseCaseAn(ar);
-    
+			assert(ar + R_ar == ar + [R_ar[0]]);
      } else {
     calc{
     An(ar + R_ar);
@@ -77,17 +80,19 @@ lemma HomAn(ar : seq<bool>, R_ar : seq<bool>)
 } // End lemma.
 
 lemma BaseCaseBn(ar : seq<bool>, R_ar : seq<bool>)
-  ensures Bn(ar) == BnJoin(Aux_1(ar), Bn(ar), An(ar), Aux_1([R_ar[0]]), Bn([R_ar[0]]), An([R_ar[0]]))
+  requires |ar| >= 1 && |R_ar| >= 1
+  ensures Bn(ar + [R_ar[0]]) == BnJoin(Aux_1(ar), Bn(ar), An(ar), Aux_1([R_ar[0]]), Bn([R_ar[0]]), An([R_ar[0]]))
   {}
 
 lemma HomBn(ar : seq<bool>, R_ar : seq<bool>)
+  requires |ar| >= 1 && |R_ar| >= 1
   ensures Bn(ar + R_ar) == BnJoin(Aux_1(ar), Bn(ar), An(ar), Aux_1(R_ar), Bn(R_ar), An(R_ar))
   {
-    if R_ar == [] 
+    if |R_ar| == 1
     {
-    assert(ar + [] == ar);
+    assert(ar + R_ar == ar + [R_ar[0]]);
     BaseCaseBn(ar, R_ar);
-    
+
      } else {
     calc{
     Bn(ar + R_ar);
@@ -100,4 +105,3 @@ lemma HomBn(ar : seq<bool>, R_ar : seq<bool>)
     } // End calc.
   } // End else.
 } // End lemma.
-
