ocamllibs/dafny_examples/Example_count_1s.dfy
@@ -3,19 +3,21 @@ function DfLength(s: seq<int>): int
 
 function Aux_0(a : seq<bool>): bool
 requires |a| >= 1
-{ if |a| == 1 then  a[0] else  a[0] 
+{
+  if |a| == 1 then a[0] else a[0]
 }
 
 function F(a : seq<bool>): bool
-{ if a == [] then  false else  a[|a|-1] 
+{
+  if a == [] then false else a[|a|-1]
 }
 
 function Cnt(a : seq<bool>): int
-{ if a == [] then
+{
+  if a == [] then
     0
-   else 
-   (Cnt(a[..|a|-1]) + (if (a[|a|-1] && (! F(a[..|a|-1]))) then 1 else 0))
-   
+    else
+    (Cnt(a[..|a|-1]) + (if (a[|a|-1] && (! F(a[..|a|-1]))) then 1 else 0))
 }
 
 function Aux_0Join(leftAux_0 : bool, rightAux_0 : bool): bool
@@ -35,13 +37,20 @@ function CntJoin(leftAux_0 : bool, leftCnt : int, leftF : bool, rightAux_0 : boo
 }
 
 
+lemma BaseCaseAux_0(a : seq<bool>, R_a : seq<bool>)
+  requires |a| >= 1 && |R_a| >= 1
+  ensures Aux_0(a + [R_a[0]]) == Aux_0Join(Aux_0(a), Aux_0([R_a[0]]))
+  {}
+
 lemma HomAux_0(a : seq<bool>, R_a : seq<bool>)
+  requires |a| >= 1 && |R_a| >= 1
   ensures Aux_0(a + R_a) == Aux_0Join(Aux_0(a), Aux_0(R_a))
   {
-    if |R_a| == 1 
+    if |R_a| == 1
     {
     assert(a + R_a == a + [R_a[0]]);
-    
+    BaseCaseAux_0(a, R_a);
+
      } else {
     calc{
     Aux_0(a + R_a);
@@ -51,18 +60,14 @@ lemma HomAux_0(a : seq<bool>, R_a : seq<bool>)
   } // End else.
 } // End lemma.
 
-lemma BaseCaseF(a : seq<bool>)
-  ensures F(a) == FJoin(F(a), F([]))
-  {}
 
 lemma HomF(a : seq<bool>, R_a : seq<bool>)
+	requires |R_a| >= 1
   ensures F(a + R_a) == FJoin(F(a), F(R_a))
   {
-    if R_a == [] 
+    if |R_a| == 1
     {
-    assert(a + [] == a);
-    BaseCaseF(a);
-    
+			assert(a + R_a == a + [R_a[0]]);
      } else {
     calc{
     F(a + R_a);
@@ -73,17 +78,19 @@ lemma HomF(a : seq<bool>, R_a : seq<bool>)
 } // End lemma.
 
 lemma BaseCaseCnt(a : seq<bool>, R_a : seq<bool>)
-  ensures Cnt(a) == CntJoin(Aux_0(a), Cnt(a), F(a), Aux_0([R_a[0]]), Cnt([R_a[0]]), F([R_a[0]]))
+  requires |a| >= 1 && |R_a| >= 1
+  ensures Cnt(a + [R_a[0]]) == CntJoin(Aux_0(a), Cnt(a), F(a), Aux_0([R_a[0]]), Cnt([R_a[0]]), F([R_a[0]]))
   {}
 
 lemma HomCnt(a : seq<bool>, R_a : seq<bool>)
+  requires |a| >= 1 && |R_a| >= 1
   ensures Cnt(a + R_a) == CntJoin(Aux_0(a), Cnt(a), F(a), Aux_0(R_a), Cnt(R_a), F(R_a))
   {
-    if R_a == [] 
+    if |R_a| == 1
     {
-    assert(a + [] == a);
+    assert(a + R_a == a + [R_a[0]]);
     BaseCaseCnt(a, R_a);
-    
+
      } else {
     calc{
     Cnt(a + R_a);
@@ -96,4 +103,3 @@ lemma HomCnt(a : seq<bool>, R_a : seq<bool>)
     } // End calc.
   } // End else.
 } // End lemma.
-
